Preliminary support for loops returning two ADTs

src/FiatToFacade/Compiler/ADTs/Folds.v
@@ -38,13 +38,371 @@ Ltac loop_body_prereqs :=
             eassumption
           | match goal with
               | [ H: AllADTs ?state ?adts |- AllADTs _ _ ] =>
-                rewrite H, AllADTs_swap_left_iff by congruence;
-                  apply AllADTs_chomp_remove;
-                  trickle_deletion;
-                  apply AllADTs_chomp;
-                  reflexivity
-            end ]
+                rewrite H;
+                  first [ rewrite AllADTs_swap_left_iff by congruence;
+                          apply AllADTs_chomp_remove;
+                          trickle_deletion;
+                          apply AllADTs_chomp;
+                          reflexivity
+                        | repeat (rewrite <- AllADTs_swap_iff;
+                                  [ apply AllADTs_chomp_remove; trickle_deletion
+                                  | solve [eauto] ]);
+                          rewrite add_add_add';
+                          reflexivity ]
+            end 
+          ]
   ].
+
+Definition compile_fold_base_pair_adt :
+  forall {env},
+  forall {acc_type} {wadt1 wadt2},
+  forall {vseq vadt1 vadt2: StringMap.key},
+  forall {thead tis_empty: StringMap.key},
+  forall {fpop fempty},
+  forall {loop compiled_loop},
+  forall {knowledge scas adts},
+    @ADTPairLoopBodyOk env acc_type loop compiled_loop knowledge scas adts
+                    vseq vadt1 vadt2 thead tis_empty wadt1 wadt2 ->
+    GLabelMap.find fempty env = Some (Axiomatic List_empty) ->
+    GLabelMap.find fpop env  = Some (Axiomatic List_pop) ->
+    vadt1 <> vadt2 ->
+    vadt1 <> vseq ->
+    vadt1 <> tis_empty ->
+    vadt2 <> vseq ->
+    vadt2 <> tis_empty ->
+    thead <> vadt1 ->
+    thead <> vadt2 ->
+    thead <> vseq ->
+    tis_empty <> vseq ->
+    ~ StringMap.In thead adts ->
+    ~ StringMap.In tis_empty adts ->
+    ~ StringMap.In vseq scas ->
+    forall seq (init: acc_type), 
+      refine (@Prog _ env knowledge
+                    (scas)
+                    ([tis_empty >sca> 1]::scas)
+                    ([vadt1 >adt> wadt1 init]::[vadt2 >adt> wadt2 init]::[vseq >adt> List seq]::adts)
+                    ([vadt1 >adt> wadt1 (List.fold_left loop seq init)]::[vadt2 >adt> wadt2 (List.fold_left loop seq init)]::[vseq >adt> List nil]::adts))
+             (ret (Fold thead tis_empty vseq fpop fempty compiled_loop)).
+Proof.
+  unfold ADTPairLoopBodyOk, ADTPairLoopBodyProgCondition, Prog, ProgOk, refine; unfold_coercions;
+  induction seq as [ | a seq ]; intros;
+  [ | specialize (fun init => IHseq init _ (eq_ret_compute _ _ _ (eq_refl))) ];
+  constructor; intros; destruct_pairs;
+  split;
+  inversion_by computes_to_inv;
+  subst;
+  scas_adts_mapsto.
+ 
+  (** Safe **)
+  constructor.
+  split; intros.
+
+  (* Call is safe *)
+  
+  eapply safe_call_1;
+    first [ eassumption
+          | symmetry; eassumption (* TODO: Can be removed *)
+          | simpl; eexists; reflexivity
+          | map_iff_solve intuition ].
+
+  (* (Non-running) loop is safe *)
+
+  compile_fold_induction_is_empty_call.
+  eapply SafeWhileFalse.
+  eapply BoolToW_eval;
+    [ reflexivity | rewrite_Eq_in_goal; map_iff_solve intuition ].
+
+  (** RunsTo **)
+  unfold Fold; intros; do 2 inversion_facade;
+  try compile_fold_induction_is_empty_call;
+  simpl;
+  scas_adts_mapsto;
+  mapsto_eq_add;
+  try (match goal with
+         | [ H: is_true _ _ |- _ ] => apply is_true_eq in H
+       end; auto_mapsto_unique).
+
+  split; rewrite_Eq_in_goal; map_iff_solve idtac.
+  apply SomeSCAs_chomp; assumption.
+  apply add_adts_pop_sca; [ map_iff_solve intuition | assumption ].
+
+  (** Induction's safety **)
+  constructor; split.
+
+  (* Call safe *)
+  eapply safe_call_1;
+    first [ eassumption
+          | symmetry; eassumption
+          | simpl; eexists; reflexivity
+          | map_iff_solve intuition ].
+
+  (* Loop safe *)
+  intros.
+  compile_fold_induction_is_empty_call; try discriminate.
+  mapsto_eq_add.
+  
+  constructor;
+    [ unfold_coercions;
+      rewrite is_true_eq;
+      assumption | | ].
+  
+  constructor; split.
+
+  (* Pop safe *)
+  assert (st' [vseq >> ADT (List (a :: seq))]) 
+    by (rewrite_Eq_in_goal; map_iff_solve intuition).
+
+  eapply safe_call_1.
+  eassumption.
+  eassumption.
+  rewrite_Eq_in_goal.
+  apply add_adts_pop_sca;
+    [ | eassumption | .. ];
+    map_iff_solve intuition.
+  map_iff_solve intuition.
+  simpl. eexists. eexists. reflexivity.
+
+  intros.
+  constructor.
+  (* Loop body + next statement safe *)
+
+  repeat match goal with
+           | [ H: (forall acc head seq initial_state,
+                     _ -> (forall final_state, RunsTo _ ?compiled_loop _ _ -> _))
+               |- context[RunsTo _ ?compiled_loop ?initial _] ] =>
+             specialize (fun p final => H init a seq initial p final);
+               match type of H with
+                 | ?cond -> _ => try pose cond as prereq
+               end
+         end.
+
+  assert (prereq) as prereqs; unfold prereq in *; clear prereq.
+  loop_body_prereqs.
+  
+  (* Loop body *)
+  split.
+  eauto.
+
+  (* next statement *)
+  intros.
+  repeat match goal with
+           | [ H: _ -> (forall final_state, _ -> _),
+               H': RunsTo _ compiled_loop _ _ |- _ ] => specialize (H prereqs _ H')
+         end.
+
+  
+  scas_adts_mapsto.
+  eapply safe_call_1; try eassumption.
+  map_iff_solve congruence.
+  simpl; eexists; reflexivity.
+
+  (* Actual loop induction *)
+  intros.
+
+  do 2 inversion_facade.
+
+  repeat match goal with
+           | [ H: (forall acc head seq initial_state,
+                     _ -> (forall final_state, RunsTo _ ?compiled_loop _ _ -> _)),
+               H': RunsTo _ ?compiled_loop ?initial _ |- _ ] =>
+             specialize (fun p final => H init a seq initial p final);
+               match type of H with
+                 | ?cond -> _ => try pose cond as prereq
+               end
+         end.
+
+  assert (prereq) as prereqs; unfold prereq in *; clear prereq.
+  loop_body_prereqs.
+
+  repeat match goal with
+           | [ H: _ -> (forall final_state, _ -> _),
+               H': RunsTo _ compiled_loop _ _ |- _ ] => specialize (H prereqs _ H')
+         end.
+
+  match goal with
+    | [ H: RunsTo _ _ _ ?st |- Safe env _ ?st ] => apply (SafeSeq_inv H)
+  end.
+  specialize (IHseq (loop init a)); inversion_by computes_to_inv.
+  match goal with
+    | [ H: context[Fold] |- _ ] => unfold Fold in H; apply H
+  end.
+
+  tauto.
+
+  (* Induction case for the loop *)
+  simpl; intros.
+  specialize (IHseq (loop init a)); inversion_by computes_to_inv.
+
+  (* initial_state is at the very beginning of the loop.  We need to unfold one
+     iteration first, and then deduce the new states *)
+
+  unfold Fold in *.
+  inversion_facade.
+
+  (* TODO: This is a dupe of part of the loop_body_prereqs code *)
+  match goal with
+    | [ H: RunsTo _ (Call _ _ _) _ _ |- _ ] =>
+      eapply runsto_is_empty in H; eauto;
+      destruct H as [ret (ret_val & state_eq)];
+      destruct ret_val; destruct_pairs; try discriminate (* Remove the list empty case *)
+  end.
+
+  assert (is_true st' (tis_empty = 0)%facade) by
+      (unfold_coercions; rewrite is_true_eq;
+       rewrite_Eq_in_goal;
+       map_iff_solve intuition). (* TODO this should be a lemma *)
+
+  inversion_facade; try (exfalso; eapply true_and_false; eassumption).
+  
+  (* Unfold one loop iteration, but keep the last statement, and merge it back at the beginning of the while, to recreate the induction condition. *)
+
+  repeat match goal with
+           | [ H: RunsTo _ (Seq _ _) _ _ |- _ ] =>
+             inversion_clear' H
+         end.
+
+  (* Copied from earlier *)
+  repeat match goal with
+           | [ H: (forall acc head seq initial_state,
+                     _ -> (forall final_state, RunsTo _ ?compiled_loop _ _ -> _)),
+               H': RunsTo _ ?compiled_loop ?initial _ |- _ ] =>
+             specialize (fun p final => H init a seq initial p final);
+               match type of H with
+                 | ?cond -> _ => try pose cond as prereq
+               end
+         end.
+
+  assert (prereq) as prereqs; unfold prereq in *; clear prereq.
+  loop_body_prereqs.
+
+  repeat match goal with
+           | [ H: _ -> (forall final_state, _ -> _),
+               H': RunsTo _ compiled_loop _ _ |- _ ] => specialize (H prereqs _ H'); pose H
+         end.
+  (* </Copied> *)
+
+  (* Stick together the last statement and the body of the loop *)
+  match goal with
+    | [ Hlast: RunsTo _ _ ?initial_state ?st, Hloop: RunsTo _ (DFacade.While _ _) ?st ?final_state |- _ ] =>
+      pose proof (RunsToSeq Hlast Hloop)
+  end.
+  specialize_states.
+  split; intuition.
+Qed.
+
+Lemma PickComputes_inv: forall {A} (x: A) P,
+                          computes_to (Pick (fun x => P x)) x -> P x.
+Proof.
+  intros; inversion_by computes_to_inv; assumption.
+Qed.
+
+Lemma map_add_remove_swap :
+  forall {elt} k1 k2 v m,
+    k1 <> k2 ->
+    @StringMap.Equal elt
+                     ([k1 >> v]::(StringMap.remove k2 m))
+                     (StringMap.remove k2 ([k1 >> v]::m)).
+Proof.
+  intros; red; intros k3.
+  map_iff_solve idtac.
+
+  repeat (rewrite ?StringMapFacts.add_o;
+          rewrite ?StringMapFacts.remove_o).
+  destruct (StringMap.E.eq_dec k1 k3), (StringMap.E.eq_dec k2 k3);
+    subst; congruence.
+Qed.
+
+Ltac autospecialize_simple :=
+  repeat match goal with
+           | [ H: ?a -> _, H': ?a |- _ ] =>
+             match (type of a) with
+               | Prop => specialize (H H')
+             end
+         end.
+
+Lemma compile_fold_pair_adt :
+  forall env,
+  forall acc_type wadt1 wadt2,
+  forall vseq vadt1 vadt2: StringMap.key,
+  forall thead tis_empty: StringMap.key,
+  forall fpop fempty,
+  forall loop,
+  forall knowledge scas adts,
+    GLabelMap.find fempty env = Some (Axiomatic List_empty) ->
+    GLabelMap.find fpop env  = Some (Axiomatic List_pop) ->
+    vadt1 <> vadt2 ->
+    vadt1 <> vseq ->
+    vadt1 <> tis_empty ->
+    vadt2 <> vseq ->
+    vadt2 <> tis_empty ->
+    thead <> vadt1 ->
+    thead <> vadt2 ->
+    thead <> vseq ->
+    tis_empty <> vseq ->
+    ~ StringMap.In thead adts ->
+    ~ StringMap.In tis_empty adts ->
+    ~ StringMap.In vseq scas ->
+    ~ StringMap.In tis_empty scas ->
+    forall seq init, 
+      refine (@Prog _ env knowledge
+                    scas scas
+                    ([vseq >adt> List seq]::adts)
+                    ([vadt1 >adt> wadt1 (List.fold_left loop seq init)]
+                       ::[vadt2 >adt> wadt2 (List.fold_left loop seq init)]
+                       ::[vseq >adt> List nil]::adts))
+             (cloop <- { cloop | @ADTPairLoopBodyOk env acc_type loop cloop knowledge
+                                                    scas adts vseq vadt1 vadt2 thead tis_empty wadt1 wadt2 };
+              pinitadt1 <- (@Prog _ env knowledge
+                                 scas scas
+                                 ([vseq >adt> List seq]::adts)
+                                 ([vadt2 >adt> wadt2 init]::[vseq >adt> List seq]::adts));
+              pinitadt2 <- (@Prog _ env knowledge
+                                 scas scas
+                                 ([vadt2 >adt> wadt2 init]::[vseq >adt> List seq]::adts)
+                                 ([vadt1 >adt> wadt1 init]::[vadt2 >adt> wadt2 init]::[vseq >adt> List seq]::adts));
+              ret (pinitadt1; pinitadt2; Fold thead tis_empty vseq fpop fempty cloop)%facade)%comp.
+Proof.
+  unfold refine; intros.
+  inversion_by computes_to_inv;
+    subst;
+    constructor;
+    match goal with
+      | [ H: _ |- _ ] => apply PickComputes_inv in H; unfold ProgOk in H
+    end. unfold ProgOk in * ;
+    intros; destruct_pairs;
+    specialize_states;
+    destruct_pairs.
+
+  match goal with
+    | [ H: context[ADTPairLoopBodyOk], H': context[GLabelMap.find], H'': context[GLabelMap.find] |- _ ] =>
+      pose proof (compile_fold_base_pair_adt H H' H'')
+  end.
+
+  autospecialize_simple.
+  unfold refine, Prog, ProgOk in *.
+
+  match goal with
+    | [ H: _ -> _ -> _ |- _ ] => specialize (H seq init _ (eq_ret_compute _ _ _ (eq_refl)))
+  end.
+  inversion_by computes_to_inv.
+  
+  split.
+
+  (* Safe *)
+  repeat (safe_seq; intros).
+  specialize_states; intuition.
+  
+  (* RunsTo *)
+  intros; destruct_pairs.
+  repeat inversion_facade.
+  specialize_states.
+  split; [ | intuition ].
+  
+  (* Tricks to get rid of is_empty *)
+  rewrite (not_in_remove_eq tis_empty scas); eauto.
+  eapply SomeSCAs_remove; eauto.
+Qed.
 
 Definition compile_fold_base_pair :
   forall {env},
@@ -741,36 +1099,6 @@ Proof.
   specialize_states.
   split; intuition.
 Qed.
-
-Lemma PickComputes_inv: forall {A} (x: A) P,
-                          computes_to (Pick (fun x => P x)) x -> P x.
-Proof.
-  intros; inversion_by computes_to_inv; assumption.
-Qed.
-
-Lemma map_add_remove_swap :
-  forall {elt} k1 k2 v m,
-    k1 <> k2 ->
-    @StringMap.Equal elt
-                     ([k1 >> v]::(StringMap.remove k2 m))
-                     (StringMap.remove k2 ([k1 >> v]::m)).
-Proof.
-  intros; red; intros k3.
-  map_iff_solve idtac.
-
-  repeat (rewrite ?StringMapFacts.add_o;
-          rewrite ?StringMapFacts.remove_o).
-  destruct (StringMap.E.eq_dec k1 k3), (StringMap.E.eq_dec k2 k3);
-    subst; congruence.
-Qed.
-
-Ltac autospecialize_simple :=
-  repeat match goal with
-           | [ H: ?a -> _, H': ?a |- _ ] =>
-             match (type of a) with
-               | Prop => specialize (H H')
-             end
-         end.
 
 Lemma compile_fold_sca :
   forall env,
