src/FiatToFacade/Loop.v
@@ -51,3 +51,20 @@ Definition PairLoopBodyOk
   forall acc (head: W) (seq: list W),
     @PairLoopBodyProgCondition env acc_type loop compiled_loop knowledge scas adts
                                vseq vsca vadt thead tis_empty acc wsca wadt head seq.
+
+Definition ADTPairLoopBodyProgCondition
+           env {acc_type} loop compiled_loop knowledge scas adts
+           (vseq vadt1 vadt2 thead tis_empty: StringMap.key) (acc: acc_type) wadt1 wadt2 (head: W) (seq: list W) :=
+  @ProgOk _ env compiled_loop knowledge
+          ([thead >sca> head]::[tis_empty >sca> 0]::scas)
+          (scas)
+          ([vadt1 >adt> wadt1 acc]::[vadt2 >adt> wadt2 acc]::[vseq >adt> List seq]::adts)
+          ([vadt1 >adt> wadt1 (loop acc head)]::[vadt2 >adt> wadt2 (loop acc head)]::[vseq >adt> List seq]::adts).
+
+Definition ADTPairLoopBodyOk
+           env {acc_type} loop compiled_loop knowledge scas adts
+           (vseq vadt1 vadt2 thead tis_empty: StringMap.key) wadt1 wadt2 :=
+  forall acc (head: W) (seq: list W),
+    @ADTPairLoopBodyProgCondition env acc_type loop compiled_loop knowledge scas adts
+                                  vseq vadt1 vadt2 thead tis_empty acc wadt1 wadt2 head seq.
+
