src/FiatToFacade/Compiler/Pairs.v
@@ -89,3 +89,34 @@ Proof.
     scas_adts_mapsto.
   intuition.
 Qed.
+
+
+Lemma compile_adt_pair :
+  forall {pair_type av env knowledge} vadt1 vadt2 {wadt1 wadt2: pair_type -> av} adts inter_adts final_adts scas pair,
+    refine
+    (@Prog av env knowledge
+           scas scas
+           adts ([vadt2 >adt> wadt2 pair]::final_adts))
+    (p <- (@Prog av env knowledge
+                 scas scas
+                 adts ([vadt1 >adt> wadt1 pair]::[vadt2 >adt> wadt2 pair]::inter_adts));
+     cleanup <- (@Prog av env knowledge
+                       scas scas
+                       ([vadt1 >adt> wadt1 pair]::[vadt2 >adt> wadt2 pair]::inter_adts)
+                       ([vadt2 >adt> wadt2 pair]::final_adts));
+     ret (p; cleanup)%facade)%comp.
+Proof.
+  unfold refine, Prog, ProgOk; unfold_coercions; intros.
+  inversion_by computes_to_inv; constructor;
+  split; subst; destruct_pairs.
+
+  repeat (safe_seq; intros).
+  specialize_states.
+  assumption.
+
+  intros;
+    repeat inversion_facade;
+    specialize_states;
+    scas_adts_mapsto.
+  intuition.
+Qed.
